cava/Examples.v
@@ -23,6 +23,9 @@ Require Import Program.Basics.
 From Coq Require Import Bool.Bool.
 From Coq Require Import Ascii String.
 From Coq Require Import Lists.List.
+From Coq Require Import ZArith.
+From Coq Require Import extraction.ExtrHaskellZInteger.
+From Coq Require Import extraction.ExtrHaskellString.
 Import ListNotations.
 
 Require Import Hask.Control.Monad.
@@ -41,7 +44,7 @@ Eval simpl in fst ((inv true) tt).
 Eval simpl in fst ((and2 (false, false)) tt).
 Eval simpl in fst ((and2 (true, true)) tt).
 
-Eval cbv in ((inv 0) (mkCavaState 1 [] [] [])).
+Eval cbv in ((inv (0%Z)) (mkCavaState (1%Z) [] [] [])).
 
 (* NAND gate example. Fist, let's define an overloaded NAND gate
    description. *)
@@ -54,7 +57,7 @@ Eval simpl in fst ((nand2 (true, true)) tt).
 
 (* Generate a circuit graph representation for the NAND gate using the
    netlist interpretatin. *)
-Eval cbv in ((nand2 (0, 1)) (mkCavaState 2 [] [] [])).
+Eval cbv in ((nand2 (0%Z, 1%Z)) (mkCavaState (2%Z) [] [] [])).
 
 Definition nand2Top {m t} `{CavaTop m t} :=
   a <- input "a" ;
